src/Word.v
@@ -62,7 +62,7 @@ Fixpoint wordToN sz (w : word sz) : N :=
   match w with
     | WO => 0
     | WS false w' => 2 * wordToN w'
-    | WS true w' => Nsucc (2 * wordToN w')
+    | WS true w' => N.succ (2 * wordToN w')
   end%N.
 Arguments wordToN : simpl nomatch.
 
@@ -1115,7 +1115,7 @@ Definition wordBin (f : N -> N -> N) sz (x y : word sz) : word sz :=
 
 Definition wplus := wordBin Nplus.
 Definition wmult := wordBin Nmult.
-Definition wdiv := wordBin Ndiv.
+Definition wdiv := wordBin N.div.
 Definition wmod := wordBin Nmod.
 Definition wmult' sz (x y : word sz) : word sz := 
   split2 sz sz (NToWord (sz + sz) (Nmult (wordToN x) (wordToN y))).
@@ -2085,9 +2085,9 @@ Fixpoint wordToZ sz (w : word sz) : Z :=
 
 (** * Comparison Predicates and Deciders **)
 Definition wlt sz (l r : word sz) : Prop :=
-  Nlt (wordToN l) (wordToN r).
+  N.lt (wordToN l) (wordToN r).
 Definition wslt sz (l r : word sz) : Prop :=
-  Zlt (wordToZ l) (wordToZ r).
+  Z.lt (wordToZ l) (wordToZ r).
 
 Notation "w1 > w2" := (@wlt _ w2%word w1%word) : word_scope.
 Notation "w1 >= w2" := (~(@wlt _ w1%word w2%word)) : word_scope.
@@ -2101,7 +2101,7 @@ Notation "w1 '<s=' w2" := (~(@wslt _ w2%word w1%word)) (at level 70, w2 at next 
 
 Definition wlt_dec : forall sz (l r : word sz), {l < r} + {l >= r}.
   refine (fun sz l r => 
-    match Ncompare (wordToN l) (wordToN r) as k return Ncompare (wordToN l) (wordToN r) = k -> _ with
+    match N.compare (wordToN l) (wordToN r) as k return N.compare (wordToN l) (wordToN r) = k -> _ with
       | Lt => fun pf => left _ _
       | _ => fun pf => right _ _
     end (refl_equal _));
@@ -2110,7 +2110,7 @@ Defined.
 
 Definition wslt_dec : forall sz (l r : word sz), {l <s r} + {l >s= r}.
   refine (fun sz l r => 
-    match Zcompare (wordToZ l) (wordToZ r) as c return Zcompare (wordToZ l) (wordToZ r) = c -> _ with
+    match Z.compare (wordToZ l) (wordToZ r) as c return Z.compare (wordToZ l) (wordToZ r) = c -> _ with
       | Lt => fun pf => left _ _
       | _ => fun pf => right _ _
     end (refl_equal _));
@@ -2139,19 +2139,19 @@ Qed.
 Lemma lt_le : forall sz (a b : word sz),
   a < b -> a <= b.
 Proof.
-  unfold wlt, Nlt. intros. intro. rewrite <- Ncompare_antisym in H0. rewrite H in H0. simpl in *. congruence.
+  unfold wlt, N.lt. intros. intro. rewrite <- N.compare_antisym in H0. rewrite H in H0. simpl in *. congruence.
 Qed.
 Lemma eq_le : forall sz (a b : word sz),
   a = b -> a <= b.
 Proof.
-  intros; subst. unfold wlt, Nlt. rewrite Ncompare_refl. congruence.
+  intros; subst. unfold wlt, N.lt. rewrite N.compare_refl. congruence.
 Qed.
 Lemma wordToN_inj : forall sz (a b : word sz),
   wordToN a = wordToN b -> a = b.
 Proof.
   induction a; intro b0; rewrite (shatter_word b0); intuition.
   destruct b; destruct (whd b0); intros; unfold wordToN in H; fold wordToN in H.
-  f_equal. eapply IHa. eapply Nsucc_inj in H.
+  f_equal. eapply IHa. eapply N.succ_inj in H.
   destruct (wordToN a); destruct (wordToN (wtl b0)); simpl in H; try congruence.
   destruct (wordToN (wtl b0)); destruct (wordToN a); inversion H.
   destruct (wordToN (wtl b0)); destruct (wordToN a); inversion H.
@@ -2196,10 +2196,10 @@ Lemma le_neq_lt : forall sz (a b : word sz),
   b <= a -> a <> b -> b < a.
 Proof.
   intros; destruct (wlt_dec b a); auto.
-  elimtype False. apply H0. unfold wlt, Nlt in *.
-  eapply wordToN_inj. eapply Ncompare_eq_correct.
+  elimtype False. apply H0. unfold wlt, N.lt in *.
+  eapply wordToN_inj. eapply N.compare_eq_correct.
   case_eq ((wordToN a ?= wordToN b)%N); auto; try congruence.
-  intros. rewrite <- Ncompare_antisym in n. rewrite H1 in n. simpl in *. congruence.
+  intros. rewrite <- N.compare_antisym in n. rewrite H1 in n. simpl in *. congruence.
 Qed.
 
 
@@ -2283,7 +2283,7 @@ Proof.
   destruct x.
   simpl in *; omega.
   simpl in *.
-  apply Nlt_out in H.
+  apply N.lt_out in H.
   autorewrite with N in *.
   rewrite Npow2_nat in *.
   generalize dependent (x * pow2 sz).
@@ -2334,7 +2334,7 @@ Proof.
   intros.
   unfold wlt in H.
   repeat rewrite wordToN_nat in *.
-  apply Nlt_out in H.
+  apply N.lt_out in H.
   repeat rewrite Nat2N.id in *.
   auto.
 Qed.
@@ -2497,7 +2497,7 @@ Proof.
   intros.
   unfold wlt.
   repeat rewrite wordToN_nat.
-  apply Nlt_in.
+  apply N.lt_in.
   repeat rewrite Nat2N.id.
   auto.
 Qed.
@@ -2556,7 +2556,7 @@ Proof.
   rewrite <- Nat.add_sub_assoc.
   omega.
 
-  apply Nat.nlt_ge.
+  apply Nat.N.lt_ge.
   unfold not in *; intros.
   apply H.
   apply lt_wlt; auto.
@@ -2873,7 +2873,7 @@ Proof.
   reflexivity.
 Qed.
 
-(* Setting an individual bit *)
+(* Setting an iN.dividual bit *)
 
 Definition wbit sz sz' (n : word sz') := natToWord sz (pow2 (wordToNat n)).
 
