src/ExtractHaskell.v
@@ -12,8 +12,18 @@ Extraction Inline PermProg.pair_args_helper.
 (* Uncomment the next line to enable eventlog-based profiling *)
 (* Extract Inlined Constant PermProg.progseq => "Profile.progseq __FILE__ __LINE__". *)
 
+Extract Inlined Constant PermProg.perm => "Prelude.Int".
+Extract Inlined Constant PermProg.perm_dec =>
+"(\x y -> if x Prelude.== y then Prelude.True else Prelude.False )".
+Extract Inlined Constant PermProg.can_access =>
+"(\x y -> case y of
+          Public -> Prelude.True
+          Private n -> if x Prelude.== n then Prelude.True else Prelude.False)".
 Extract Inlined Constant PermProg.handle => "Word.Coq_word".
 Extract Inlined Constant PermAsyncDisk.owner => "Prelude.Int".
+Extract Inlined Constant PermAsyncDisk.dummy_owner => "0".
+Extract Inlined Constant PermAsyncDisk.owner_dec =>
+"(\x y -> if x Prelude.== y then Prelude.True else Prelude.False )".
 Extract Inlined Constant PermInode.encode_tag => "Interpreter.encode_tag".
 Extract Inlined Constant PermInode.decode_tag => "Interpreter.decode_tag".
 
